src/program_proof/memkv/memkv_shard_ghost_init.v
@@ -8,40 +8,36 @@ From Perennial.program_proof.memkv Require Export memkv_shard_definitions.
 Section memkv_shard_ghost_init_proof.
 
 (* These lemmas happen *before* we get node local names (e.g. the gname for memory, crashes etc. *)
-Context `{!gooseGlobalGS Σ, erpcG Σ ShardReplyC, urpcregG Σ, kvMapG Σ}.
+Context `{!gooseGlobalGS Σ, erpcG Σ, urpcregG Σ, kvMapG Σ}.
 
 (* TODO: duplicating this specs is unfortunate, should try to unify with the set up in shard_definitions *)
 
 Definition shard_SpecList γkv γrpc : uRPCSpecList :=
-  spec_cons (is_shard_server_putSpec γkv γrpc)
-    (spec_cons (is_shard_server_conditionalPutSpec γkv γrpc)
-      (spec_cons (is_shard_server_getSpec γkv γrpc)
+  spec_cons (eRPCSpec_uRPC γrpc $ is_shard_server_putSpec γkv)
+    (spec_cons (eRPCSpec_uRPC γrpc $ is_shard_server_conditionalPutSpec γkv)
+      (spec_cons (eRPCSpec_uRPC γrpc $ is_shard_server_getSpec γkv)
         (spec_cons (is_shard_server_moveSpec γkv)
-          (spec_cons (is_shard_server_installSpec γkv γrpc)
+          (spec_cons (eRPCSpec_uRPC γrpc $ is_shard_server_installSpec γkv)
             (spec_cons (is_shard_server_freshSpec γrpc) spec_nil))))).
 
 Lemma shard_server_ghost_init host (γkv : gname) :
   host c↦ ∅ ={⊤}=∗
   ∃ γ, ⌜ γ.(kv_gn) = γkv ⌝ ∗
-       handlers_dom γ.(urpc_gn) (dom_uRPCSpecList (shard_SpecList (γ.(kv_gn)) (γ.(rpc_gn)))) ∗
+       handlers_dom γ.(urpc_gn) (dom_uRPCSpecList (shard_SpecList (γ.(kv_gn)) (γ.(erpc_gn)))) ∗
        is_shard_server host γ ∗
-       eRPCServer_own_ghost γ.(rpc_gn) ∅ ∅ ∗
-      ([∗ set] cid ∈ fin_to_set u64, is_eRPCClient_ghost γ.(rpc_gn) cid 1).
+       own_erpc_pre_server γ.(erpc_gn).
 Proof.
   iIntros "Hg".
-  iMod (make_rpc_server (R := ShardReplyC)) as (γrpc) "(#Hown&Hrpc1&Hrpc2)".
-  { set_solver. }
+  iMod (erpc_init_server_ghost) as (γrpc) "Herpc".
   iMod (handler_is_init_list host (shard_SpecList γkv γrpc) with "[Hg]") as (γ) "H".
   { simpl. set_solver. }
   { iExactEq "Hg". f_equal. }
   iDestruct "H" as "(#Hdom&#Hput&#Hcput&#Hget&#Hmove&#Hinstall&#Hfresh&_)".
 
-  set (Γsrv := {| rpc_gn := γrpc; urpc_gn := γ; kv_gn := γkv |}).
+  set (Γsrv := {| erpc_gn := γrpc; urpc_gn := γ; kv_gn := γkv |}).
   iAssert (is_shard_server host Γsrv) as "Hshard".
   {
     rewrite is_shard_server_unfold /is_shard_server_pre.
-    iSplitL.
-    { iFrame "#Hown". }
     iSplitL. { iFrame "Hput". }
     iSplitL. { iFrame "Hcput". }
     iSplitL. { iFrame "Hget". }
