src/program_proof/fencing/frontend_proof.v
@@ -342,6 +342,7 @@ Proof.
       simpl. iExists _; iFrame "#".
 
       clear Φ.
+      rewrite /impl_handler_spec.
       iIntros (??????) "!#".
       iIntros (Φ) "Hpre HΦ".
       iDestruct "Hpre" as "(Hreq_sl & Hrep & Hrep_sl & HFAISpec)".
