src/program_proof/memkv/memkv_conditional_put_proof.v
@@ -4,29 +4,26 @@ From Perennial.program_proof.memkv Require Export memkv_shard_definitions common
 
 Section memkv_conditional_put_proof.
 
-Context `{!heapGS Σ, erpcG Σ ShardReplyC, HREG: urpcregG Σ, kvMapG Σ}.
+Context `{!heapGS Σ, erpcG Σ, urpcregG Σ, kvMapG Σ}.
 
 Local Ltac Zify.zify_post_hook ::= Z.div_mod_to_equations.
 
-Lemma wp_ConditionalPutRPC (s args_ptr reply_ptr:loc) expv_sl newv_sl args γ γreq Q :
+Lemma wp_ConditionalPutRPC (s args_ptr reply_ptr:loc) expv_sl newv_sl args Q γ :
   is_KVShardServer s γ -∗
   {{{
        own_ConditionalPutRequest args_ptr expv_sl newv_sl args ∗
        (∃ dummy_rep, own_ConditionalPutReply reply_ptr dummy_rep) ∗
-       is_eRPCRequest γ.(rpc_gn) γreq (PreShardConditionalPut γ.(kv_gn) args.(CPR_Key) Q args.(CPR_ExpValue) args.(CPR_NewValue))
-                                (PostShardConditionalPut γ.(kv_gn) args.(CPR_Key) Q args.(CPR_ExpValue) args.(CPR_NewValue))
-                                {| Req_CID:=args.(CPR_CID); Req_Seq:=args.(CPR_Seq) |}
+       PreShardConditionalPut γ.(kv_gn) args.(CPR_Key) Q args.(CPR_ExpValue) args.(CPR_NewValue)
   }}}
     KVShardServer__ConditionalPutRPC #s #args_ptr #reply_ptr
   {{{
        rep, RET #();
        own_ConditionalPutReply reply_ptr rep ∗
-       (eRPCRequestStale γ.(rpc_gn) {| Req_CID:=args.(CPR_CID); Req_Seq:=args.(CPR_Seq) |} ∨
-        ∃ dummy_val, eRPCReplyReceipt γ.(rpc_gn) {| Req_CID:=args.(CPR_CID); Req_Seq:=args.(CPR_Seq) |} (mkShardReplyC rep.(CPR_Err) dummy_val rep.(CPR_Succ)))
+       PostShardConditionalPut γ.(kv_gn) args.(CPR_Key) Q args.(CPR_ExpValue) args.(CPR_NewValue) rep
   }}}.
 Proof.
   iIntros "#His_shard !#" (Φ) "Hpre HΦ".
-  iDestruct "Hpre" as "(Hargs & Hrep & #HreqInv)".
+  iDestruct "Hpre" as "(Hargs & Hrep & Hpre)".
   iNamed "Hargs". iNamed "Hrep".
 
   wp_lam.
@@ -43,452 +40,205 @@ Proof.
   wp_lam.
   wp_pures.
 
-  wp_loadField. wp_loadField.
-  wp_apply (wp_MapGet with "HlastSeqMap").
-  iIntros (seqno ok) "[%HseqGet HlastSeqMap]".
   wp_pures.
-
   wp_loadField.
+  wp_apply (wp_shardOf).
   wp_pures.
+  wp_loadField.
 
-  wp_apply (wp_and_pure ok (int.Z args.(CPR_Seq) ≤ int.Z seqno)%Z).
-  { wp_pures. by destruct ok. }
-  { iIntros "_". wp_pures. done. }
+  iDestruct (typed_slice.is_slice_small_acc with "HshardMap_sl") as "[HshardMap_sl HshardMap_sl_close]".
+  set (sid:=shardOfC args.(CPR_Key)) in *.
+
+  assert (∃ b, shardMapping !! int.nat sid = Some b) as [? ?].
+  {
+    eapply list_lookup_lt.
+    move: HshardMapLength. rewrite /sid /shardOfC /uNSHARD.
+    word.
+  }
+  wp_apply (typed_slice.wp_SliceGet with "[$HshardMap_sl]").
+  {
+    iPureIntro. done.
+  }
+  iIntros "HshardMap_sl".
+  wp_pures.
 
   wp_if_destruct.
-  { (* reply table *)
+  { (* have the shard *)
     wp_loadField.
-    wp_loadField.
-    wp_apply (map.wp_MapGet with "HlastReplyMap").
-    iIntros (reply replyOk) "[%HlookupReply HlastReplyMap]".
-    wp_pures.
+    iDestruct (is_slice_split with "Hkvss_sl") as "[Hkvss_sl Hkvss_sl_close]".
+    iDestruct (big_sepS_elem_of_acc _ _ sid with "HownShards") as "[HownShard HownShards]".
+    { set_solver. }
+    iDestruct "HownShard" as "[%Hbad|HownShard]".
+    { exfalso. done. }
+    iDestruct "HownShard" as (kvs_ptr m mv) "(HshardGhost & %Hkvs_lookup & %Hdom_kvs& HkvsMap & HvalSlices)".
+    wp_apply (slice.wp_SliceGet _ _ _ _ _ _ _ (#kvs_ptr) with "[Hkvss_sl]").
+    {
+      iFrame "Hkvss_sl".
+      iPureIntro.
+      rewrite list_lookup_fmap.
+      rewrite Hkvs_lookup.
+      done.
+    }
+    iIntros "[Hkvss_sl %Hkvs_ty]".
 
-    destruct ok; last first.
+    wp_loadField.
+    wp_apply (map.wp_MapGet with "[$HkvsMap]").
+    iIntros (value okValue) "[%HlookupVal HkvsMap]".
+    assert (value = default (slice_val Slice.nil) (mv !! args.(CPR_Key))) as ->.
+    { naive_solver. }
+    iDestruct (big_sepS_delete _ _ args.(CPR_Key) with "HvalSlices") as "[Hsrv_val_sl HvalSlices]".
+    { set_solver. }
+    iDestruct "Hsrv_val_sl" as "[%Hbad|Hsrv_val_sl]".
     { exfalso. naive_solver. }
-    apply map_get_true in HseqGet.
-    destruct Heqb as [_ HseqLe].
+    iDestruct "Hsrv_val_sl" as (q curv_sl) "[%HvalSliceRe Hsrv_val_sl]".
+    rewrite HvalSliceRe.
 
-    (* get a copy of the is_slice for the slice we're giving in reply *)
-    assert (is_Some (lastReplyMV !! args.(CPR_CID))) as [? HlastReplyMVlookup].
+    wp_loadField.
+    iMod (readonly_load with "HExpValue_sl") as (?) "HExpValue_sl'".
+    (*
+      iDestruct (is_slice_small_acc with "Hsrv_val_sl") as "[Hsrv_val_sl Hsrv_val_close]".
+     *)
+    wp_apply (wp_BytesEqual with "[$HExpValue_sl' $Hsrv_val_sl]").
+    iIntros "[_ Hsrv_val_sl]".
+
+    (* Avoid duplicating the proof of the merged control flow after this if *)
+    wp_apply (wp_If_join_evar with "[HkvsMap HKey HNewValue]").
+    { iIntros (succ Hsucc).
+      case_bool_decide as Heq; wp_pures.
+      - wp_loadField.
+        wp_loadField.
+        set (old_map := (mv, _)).
+        wp_apply (map.wp_MapInsert with "[$HkvsMap]").
+        iIntros "HkvsMap".
+        wp_pures.
+        iSplit; first done.
+        set (new_map := map.map_insert _ args.(CPR_Key) _).
+        replace (new_map) with (if succ then new_map else old_map); last by rewrite Hsucc.
+        iNamedAccu.
+      - iModIntro. iSplit; first done.
+        rewrite Hsucc.
+        iFrame. }
+    iIntros "Hjoined". iNamed "Hjoined".
+    set (succ := bool_decide (_ = _)).
+
+    wp_storeField.
+    wp_storeField.
+    iDestruct (big_sepS_delete _ _ args.(CPR_Key) with "HshardGhost") as "[Hghost HshardGhost]".
+    { set_solver. }
+    iDestruct "Hghost" as "[%Hbad|Hkvptsto]".
+    { exfalso; done. }
+
+    (* Get Q by using fupd *)
+    unfold PreShardConditionalPut.
+    iApply ncfupd_wp.
+    iMod (ncfupd_mask_subseteq _) as "Hclose"; last iMod "Hpre".
+    { done. }
+    iDestruct "Hpre" as (v0) "(Hkvptsto2 & HfupdQ)".
+    iDestruct (kvptsto_agree with "Hkvptsto Hkvptsto2") as %<-.
+    set (newv := if succ then args.(CPR_NewValue) else (default [] (m !! args.(CPR_Key)))).
+    iMod (kvptsto_update newv with "Hkvptsto Hkvptsto2") as "[Hkvptsto Hkvptsto2]".
+    iMod ("HfupdQ" with "Hkvptsto") as "Q".
+    iMod "Hclose" as "_".
+
+    iDestruct ("HshardMap_sl_close" with "HshardMap_sl") as "HshardMap_sl".
+    iModIntro.
+    wp_loadField.
+    iMod (readonly_load with "HNewValue_sl") as (?) "HNewValue_sl'".
+    wp_apply (release_spec with "[-HΦ HKey HErr HSucc Q]").
     {
-      assert (args.(CPR_CID) ∈ dom (gset u64) lastSeqM).
-      { by eapply elem_of_dom_2. }
-      assert (args.(CPR_CID) ∈ dom (gset u64) lastReplyMV).
-      { rewrite -HlastReplyMVdom in H1. done. }
-      apply elem_of_dom.
-      done.
+      iFrame "HmuInv Hlocked".
+      iNext.
+      iExists _,_,_, _, _, _.
+      iFrame.
+      iSplitL ""; first done.
+      iSplitL ""; first done.
+      iApply "HownShards".
+      iRight.
+      iExists _, _, _.
+      iFrame.
+      instantiate (1:=(if succ then <[args.(CPR_Key):=args.(CPR_NewValue)]> m else m)).
+      iSplitL "HshardGhost Hkvptsto2".
+      {
+        iApply (big_sepS_delete _ _ args.(CPR_Key) with "[-]").
+        { set_solver. }
+        iSplitL "Hkvptsto2".
+        {
+          iRight.
+          destruct succ.
+          * rewrite lookup_insert. iFrame.
+          * iFrame.
+        }
+        iApply (big_sepS_impl with "HshardGhost").
+        iModIntro; iIntros.
+        destruct succ.
+        * rewrite lookup_insert_ne; last first.
+          { set_solver. }
+          iFrame.
+        * iFrame.
+      }
+      iSplitL ""; first done.
+      iSplitL ""; last first.
+      { iSplitL "HkvsMap".
+        { instantiate (1:=if succ then _ else _).
+          destruct succ; done. }
+        iApply (big_sepS_delete _ _ args.(CPR_Key) with "[-]").
+        { set_solver. }
+        simpl. iSplitL "HNewValue_sl' Hsrv_val_sl".
+        {
+          simpl. iRight. destruct succ.
+          - iExists _, newv_sl.
+            rewrite lookup_insert.
+            rewrite lookup_insert.
+            eauto with iFrame.
+          - iExists _, curv_sl.
+            eauto with iFrame.
+        }
+        iApply (big_sepS_impl with "HvalSlices").
+        iModIntro.
+        iIntros.
+        destruct succ.
+        * rewrite ?lookup_insert_ne; last first.
+          { set_solver. }
+          { set_solver. }
+          iFrame.
+        * iFrame.
+      }
+      destruct succ; rewrite ?dom_insert_L; iPureIntro; congruence.
     }
-
-    iDestruct (big_sepM2_lookup_iff with "HlastReply_structs") as %Hdom.
-    assert (is_Some (lastReplyM !! args.(CPR_CID))) as [? HlastReplyMlookup].
-    { apply Hdom. naive_solver. }
-
-    iDestruct (big_sepM2_lookup_acc _ _ _ args.(CPR_CID) with "HlastReply_structs") as "[HlastReply_struct HlastReply_structs]".
+    wp_pures. iApply "HΦ". iModIntro.
+    iSplitL "HErr HSucc".
     {
-      done.
+      instantiate (1:=mkConditionalPutReplyC _ _).
+      iFrame.
     }
-    {
-      done.
-    }
+    iRight.
+    iSimpl.
+    iFrame "Q".
+    done.
+  }
+  { (* don't have shard *)
+    wp_storeField.
 
-    iDestruct "HlastReply_struct" as (srv_val_sl ?) "[%Hx Hsrv_val_sl]".
-    assert (x = reply) as ->.
+    wp_loadField.
+    iSpecialize ("HshardMap_sl_close" with "HshardMap_sl").
+    wp_apply (release_spec with "[-HΦ HKey HErr HSucc Hpre]").
     {
-      unfold map.map_get in HlookupReply.
-      rewrite HlastReplyMVlookup in HlookupReply.
-      naive_solver.
-    }
-
-    rewrite Hx.
-    iDestruct "Hsrv_val_sl" as "[Hsrv_val_sl Hrep_val_sl]".
-    iSpecialize ("HlastReply_structs" with "[Hsrv_val_sl]").
-    {
-      iExists _, _.
+      iFrame "HmuInv Hlocked".
+      iNext.
+      iExists _,_,_, _, _, _.
       iFrame.
       done.
     }
-    wp_storeField.
-    wp_storeField.
-
-    (* now split into stale/nonstale cases *)
-    destruct (Z.lt_ge_cases (int.Z args.(CPR_Seq)) (int.Z seqno)) as [Hcase|Hcase].
-    { (* Stale *)
-      iMod (smaller_seqno_stale_fact _ {| Req_CID:=_; Req_Seq:=_ |} seqno with "His_srv Hrpc") as "HH".
-      { done. }
-      { done. }
-      { done. }
-      iDestruct "HH" as "[Hrpc #Hstale]".
-      wp_loadField.
-      wp_apply (release_spec with "[-HΦ HCID HSeq HKey HExpValue_sl HNewValue_sl HErr HSucc Hrep_val_sl]").
-      {
-        iFrame "#∗".
-        iNext.
-        iExists _,_,_, _, _, _, _, _.
-        iExists _, _, _, _.
-        iFrame.
-        done.
-      }
-      wp_pures. iApply "HΦ". iModIntro.
-
-      iSplitL "HErr HSucc".
-      {
-        instantiate (1:={| CPR_Err := _ |}).
-        iFrame.
-      }
-      iLeft.
-      iFrame "#".
-    }
-    { (* Not stale *)
-      assert (seqno = args.(CPR_Seq)) by word.
-      rewrite H1 in HseqGet.
-      iMod (server_replies_to_request _ {| Req_CID:=_; Req_Seq:=_ |} with "His_srv Hrpc") as "HH".
-      { done. }
-      { done. }
-      { eexists (mkShardReplyC 0 [] false). naive_solver. }
-
-      iDestruct "HH" as "[#Hreceipt Hrpc]".
-
-      (* prove that args.(GR_CID) is in lastReplyMV (probably just add [∗ map] _ ↦ _;_ ∈ lastReplyMV ; lastSeq, True) *)
-      wp_loadField.
-      wp_apply (release_spec with "[-HΦ HCID HSeq HKey HExpValue_sl HNewValue_sl HErr HSucc Hrep_val_sl]").
-      {
-        iFrame "#∗".
-        iNext.
-        iExists _,_,_, _, _, _, _, _.
-        iExists _, _, _, _.
-        iFrame.
-        done.
-      }
-      wp_pures. iModIntro. iApply "HΦ".
-      iSplitL "HErr HSucc".
-      {
-        instantiate (1:={| CPR_Err := _ |}).
-        by iFrame.
-      }
-      iRight.
-      rewrite HlastReplyMlookup.
-      simpl.
-      destruct x0.
-      iExists _.
-      iFrame "#".
-    }
-  }
-  {
-    wp_loadField.
-    wp_loadField.
-    wp_loadField.
-    wp_apply (wp_MapInsert with "HlastSeqMap").
-    { done. }
-    iIntros "HlastSeqMap".
-
-    wp_pures.
-    wp_loadField.
-    wp_apply (wp_shardOf).
-    wp_pures.
-    wp_loadField.
-
-    iDestruct (typed_slice.is_slice_small_acc with "HshardMap_sl") as "[HshardMap_sl HshardMap_sl_close]".
-    set (sid:=shardOfC args.(CPR_Key)) in *.
-
-    assert (∃ b, shardMapping !! int.nat sid = Some b) as [? ?].
+    wp_pures. iApply "HΦ". iModIntro.
+    iSplitL "HErr HSucc".
     {
-      eapply list_lookup_lt.
-      move: HshardMapLength. rewrite /sid /shardOfC /uNSHARD.
-      word.
+      instantiate (1:=mkConditionalPutReplyC _ _).
+      iFrame.
     }
-    wp_apply (typed_slice.wp_SliceGet with "[$HshardMap_sl]").
-    {
-      iPureIntro. done.
-    }
-    iIntros "HshardMap_sl".
-    wp_pures.
-
-    assert (int.Z seqno < int.Z args.(CPR_Seq))%Z as HseqFresh.
-    {
-      simpl.
-      destruct ok.
-      {
-        intuition.
-        destruct (Z.le_gt_cases (int.Z args.(CPR_Seq)) (int.Z seqno)) as [Hineq|Hineq].
-        { naive_solver. }
-        { naive_solver. }
-      }
-      {
-        apply map_get_false in HseqGet as [_ ->].
-        simpl.
-        word.
-      }
-    }
-
-    (* get resources out of escrow before splitting into cases *)
-    iMod (server_takes_request with "HreqInv Hrpc") as "HH".
-    { done. }
-    {
-      rewrite HseqGet.
-      done.
-    }
-    iDestruct "HH" as "(Hγpre & Hpre & Hproc)".
-
-    wp_if_destruct.
-    { (* have the shard *)
-      wp_loadField.
-      iDestruct (is_slice_split with "Hkvss_sl") as "[Hkvss_sl Hkvss_sl_close]".
-      iDestruct (big_sepS_elem_of_acc _ _ sid with "HownShards") as "[HownShard HownShards]".
-      { set_solver. }
-      iDestruct "HownShard" as "[%Hbad|HownShard]".
-      { exfalso. done. }
-      iDestruct "HownShard" as (kvs_ptr m mv) "(HshardGhost & %Hkvs_lookup & %Hdom_kvs& HkvsMap & HvalSlices)".
-      wp_apply (slice.wp_SliceGet _ _ _ _ _ _ _ (#kvs_ptr) with "[Hkvss_sl]").
-      {
-        iFrame "Hkvss_sl".
-        iPureIntro.
-        rewrite list_lookup_fmap.
-        rewrite Hkvs_lookup.
-        done.
-      }
-      iIntros "[Hkvss_sl %Hkvs_ty]".
-
-      wp_loadField.
-      wp_apply (map.wp_MapGet with "[$HkvsMap]").
-      iIntros (value okValue) "[%HlookupVal HkvsMap]".
-      assert (value = default (slice_val Slice.nil) (mv !! args.(CPR_Key))) as ->.
-      { naive_solver. }
-      iDestruct (big_sepS_delete _ _ args.(CPR_Key) with "HvalSlices") as "[Hsrv_val_sl HvalSlices]".
-      { set_solver. }
-      iDestruct "Hsrv_val_sl" as "[%Hbad|Hsrv_val_sl]".
-      { exfalso. naive_solver. }
-      iDestruct "Hsrv_val_sl" as (q curv_sl) "[%HvalSliceRe Hsrv_val_sl]".
-      rewrite HvalSliceRe.
-
-      wp_loadField.
-      iMod (readonly_load with "HExpValue_sl") as (?) "HExpValue_sl'".
-      (*
-      iDestruct (is_slice_small_acc with "Hsrv_val_sl") as "[Hsrv_val_sl Hsrv_val_close]".
-       *)
-      wp_apply (wp_BytesEqual with "[$HExpValue_sl' $Hsrv_val_sl]").
-      iIntros "[_ Hsrv_val_sl]".
-
-      (* Avoid duplicating the proof of the merged control flow after this if *)
-      wp_apply (wp_If_join_evar with "[HkvsMap HKey HNewValue]").
-      { iIntros (succ Hsucc).
-        case_bool_decide as Heq; wp_pures.
-        - wp_loadField.
-          wp_loadField.
-          set (old_map := (mv, _)).
-          wp_apply (map.wp_MapInsert with "[$HkvsMap]").
-          iIntros "HkvsMap".
-          wp_pures.
-          iSplit; first done.
-          set (new_map := map.map_insert _ args.(CPR_Key) _).
-          replace (new_map) with (if succ then new_map else old_map); last by rewrite Hsucc.
-          iNamedAccu.
-        - iModIntro. iSplit; first done.
-          rewrite Hsucc.
-          iFrame. }
-      iIntros "Hjoined". iNamed "Hjoined".
-      set (succ := bool_decide (_ = _)).
-
-      wp_storeField.
-      wp_storeField.
-      iDestruct (big_sepS_delete _ _ args.(CPR_Key) with "HshardGhost") as "[Hghost HshardGhost]".
-      { set_solver. }
-      iDestruct "Hghost" as "[%Hbad|Hkvptsto]".
-      { exfalso; done. }
-
-      (* Get Q by using fupd *)
-      unfold PreShardConditionalPut.
-      iApply ncfupd_wp.
-      iMod (ncfupd_mask_subseteq _) as "Hclose"; last iMod "Hpre".
-      { done. }
-      iDestruct "Hpre" as (v0) "(Hkvptsto2 & HfupdQ)".
-      iDestruct (kvptsto_agree with "Hkvptsto Hkvptsto2") as %<-.
-      set (newv := if succ then args.(CPR_NewValue) else (default [] (m !! args.(CPR_Key)))).
-      iMod (kvptsto_update newv with "Hkvptsto Hkvptsto2") as "[Hkvptsto Hkvptsto2]".
-      iMod ("HfupdQ" with "Hkvptsto") as "Q".
-      iMod "Hclose" as "_".
-
-      (* fill in reply struct *)
-      iModIntro.
-      wp_loadField.
-      wp_loadField.
-      wp_loadField.
-      wp_loadField.
-
-      (* save reply in reply table *)
-      wp_apply (map.wp_MapInsert with "HlastReplyMap").
-      iIntros "HlastReplyMap".
-
-      wp_pures.
-
-      iMod (server_completes_request with "His_srv HreqInv Hγpre [Q] Hproc") as "HH".
-      { done. }
-      { done. }
-      { rewrite HseqGet. simpl. done. }
-      {
-        iNext.
-        iRight.
-        iFrame.
-        instantiate (1:=mkShardReplyC _ [] succ).
-        simpl.
-        eauto.
-      }
-      iDestruct "HH" as "(#Hreceipt & Hrpc)".
-
-      iDestruct ("HshardMap_sl_close" with "HshardMap_sl") as "HshardMap_sl".
-      wp_loadField.
-      iMod (readonly_load with "HNewValue_sl") as (?) "HNewValue_sl'".
-      wp_apply (release_spec with "[-HΦ HCID HSeq HKey HErr HSucc]").
-      {
-        iFrame "HmuInv Hlocked".
-        iNext.
-        iExists _,_,_, _, _, _, _, _.
-        iExists _, _, _, _.
-        iFrame.
-        iSplitL "".
-        {
-          iPureIntro.
-          simpl.
-          rewrite !dom_insert_L.
-          congruence.
-        }
-        iSplitL "HlastReply_structs".
-        {
-          iApply (big_sepM2_insert_2 with "[] HlastReply_structs").
-          { simpl.
-            iExists _, 1%Qp.
-            rewrite zero_slice_val.
-            iSplitL ""; first done.
-            iApply (typed_slice.is_slice_small_nil).
-            done.
-          }
-        }
-        iSplitL ""; first done.
-        iSplitL ""; first done.
-        iApply "HownShards".
-        iRight.
-        iExists _, _, _.
-        iFrame.
-        instantiate (1:=(if succ then <[args.(CPR_Key):=args.(CPR_NewValue)]> m else m)).
-        iSplitL "HshardGhost Hkvptsto2".
-        {
-          iApply (big_sepS_delete _ _ args.(CPR_Key) with "[-]").
-          { set_solver. }
-          iSplitL "Hkvptsto2".
-          {
-            iRight.
-            destruct succ.
-            * rewrite lookup_insert. iFrame.
-            * iFrame.
-          }
-          iApply (big_sepS_impl with "HshardGhost").
-          iModIntro; iIntros.
-          destruct succ.
-          * rewrite lookup_insert_ne; last first.
-            { set_solver. }
-            iFrame.
-          * iFrame.
-        }
-        iSplitL ""; first done.
-        iSplitL ""; last first.
-        { iSplitL "HkvsMap".
-          { instantiate (1:=if succ then _ else _).
-            destruct succ; done. }
-          iApply (big_sepS_delete _ _ args.(CPR_Key) with "[-]").
-          { set_solver. }
-          simpl. iSplitL "HNewValue_sl' Hsrv_val_sl".
-          {
-            simpl. iRight. destruct succ.
-            - iExists _, newv_sl.
-              rewrite lookup_insert.
-              rewrite lookup_insert.
-              eauto with iFrame.
-            - iExists _, curv_sl.
-              eauto with iFrame.
-          }
-          iApply (big_sepS_impl with "HvalSlices").
-          iModIntro.
-          iIntros.
-          destruct succ.
-          * rewrite ?lookup_insert_ne; last first.
-            { set_solver. }
-            { set_solver. }
-            iFrame.
-          * iFrame.
-        }
-        destruct succ; rewrite ?dom_insert_L; iPureIntro; congruence.
-      }
-      wp_pures. iApply "HΦ". iModIntro.
-      iSplitL "HErr HSucc".
-      {
-        instantiate (1:=mkConditionalPutReplyC _ _).
-        iFrame.
-      }
-      iSimpl.
-      iRight.
-      iExists [].
-      iFrame "#".
-    }
-    { (* don't have shard *)
-      wp_storeField.
-
-      iMod (server_completes_request with "His_srv HreqInv Hγpre [Hpre] Hproc") as "HH".
-      { done. }
-      { done. }
-      { rewrite HseqGet. simpl. done. }
-      {
-        iNext.
-        iLeft.
-        iFrame "Hpre".
-        instantiate (1:=mkShardReplyC 1 [] _).
-        simpl.
-        done.
-      }
-      iDestruct "HH" as "(#Hreceipt & Hrpc)".
-
-      wp_loadField.
-      wp_loadField.
-      wp_loadField.
-      wp_loadField.
-      rewrite zero_slice_val.
-
-      wp_apply (map.wp_MapInsert with "HlastReplyMap").
-      iIntros "HlastReplyMap".
-      wp_pures.
-
-      wp_loadField.
-      iSpecialize ("HshardMap_sl_close" with "HshardMap_sl").
-      wp_apply (release_spec with "[-HΦ HCID HSeq HKey HErr HSucc]").
-      {
-        iFrame "HmuInv Hlocked".
-        iNext.
-        iExists _,_,_, _, _, _, _, _.
-        iExists _, _, _, _.
-        iFrame.
-        iSplitL "".
-        { iPureIntro.
-          rewrite !dom_insert_L /=.
-          congruence. }
-        iSplitL "HlastReply_structs".
-        {
-          iApply (big_sepM2_insert_2 with "[] HlastReply_structs").
-          simpl.
-          iExists Slice.nil, 1%Qp; iFrame.
-          iSplitL ""; first done.
-          iApply (typed_slice.is_slice_small_nil).
-          done.
-        }
-        done.
-      }
-      wp_pures. iApply "HΦ". iModIntro.
-      iSplitL "HErr HSucc".
-      {
-        instantiate (1:=mkConditionalPutReplyC _ _).
-        iFrame.
-      }
-      iSimpl.
-      iRight.
-      iExists []; iFrame "Hreceipt".
-    }
+    iLeft.
+    iSimpl.
+    iFrame.
+    done.
   }
 Qed.
 
