src/program_proof/memkv/memkv_coord_ghost_init.v
@@ -8,7 +8,7 @@ From Perennial.program_proof.memkv Require Export memkv_shard_definitions memkv_
 Section memkv_coord_ghost_init_proof.
 
 (* These lemmas happen *before* we get node local names (e.g. the gname for memory, crashes etc. *)
-Context `{!gooseGlobalGS Σ, erpcG Σ ShardReplyC, urpcregG Σ, kvMapG Σ}.
+Context `{!gooseGlobalGS Σ, erpcG Σ, urpcregG Σ, kvMapG Σ}.
 
 Definition coord_SpecList γkv : uRPCSpecList :=
   spec_cons (is_coord_server_addSpec γkv)
