src/program_proof/memkv/memkv_get_proof.v
@@ -4,7 +4,7 @@ From Perennial.program_proof.memkv Require Export memkv_shard_definitions common
 
 Section memkv_shard_proof.
 
-Context `{!heapGS Σ, erpcG Σ ShardReplyC, HREG: urpcregG Σ, kvMapG Σ}.
+Context `{!heapGS Σ, erpcG Σ, urpcregG Σ, kvMapG Σ}.
 
 Lemma wp_shardOf key :
   {{{
@@ -37,25 +37,22 @@ Qed.
 
 Local Ltac Zify.zify_post_hook ::= Z.div_mod_to_equations.
 
-Lemma wp_GetRPC (s args_ptr reply_ptr:loc) args γ γreq Q :
+Lemma wp_GetRPC (s args_ptr reply_ptr:loc) args γ Q :
   is_KVShardServer s γ -∗
   {{{
        own_GetRequest args_ptr args ∗
        (∃ dummy_rep, own_GetReply reply_ptr dummy_rep) ∗
-       is_eRPCRequest γ.(rpc_gn) γreq (PreShardGet γ.(kv_gn) args.(GR_Key) Q)
-                                (PostShardGet γ.(kv_gn) args.(GR_Key) Q)
-                                {| Req_CID:=args.(GR_CID); Req_Seq:=args.(GR_Seq) |}
+       (PreShardGet γ.(kv_gn) args.(GR_Key) Q)
   }}}
     KVShardServer__GetRPC #s #args_ptr #reply_ptr
   {{{
        rep, RET #();
        own_GetReply reply_ptr rep ∗
-       (eRPCRequestStale γ.(rpc_gn) {| Req_CID:=args.(GR_CID); Req_Seq:=args.(GR_Seq) |} ∨
-        ∃ dummy_succ, eRPCReplyReceipt γ.(rpc_gn) {| Req_CID:=args.(GR_CID); Req_Seq:=args.(GR_Seq) |} (mkShardReplyC rep.(GR_Err) rep.(GR_Value) dummy_succ))
+       (PostShardGet γ.(kv_gn) args.(GR_Key) Q) rep
   }}}.
 Proof.
   iIntros "#His_shard !#" (Φ) "Hpre HΦ".
-  iDestruct "Hpre" as "(Hargs & Hrep & #HreqInv)".
+  iDestruct "Hpre" as "(Hargs & Hrep & Hpre)".
   iNamed "Hargs". iNamed "Hrep".
 
   wp_lam.
@@ -72,431 +69,161 @@ Proof.
   wp_lam.
   wp_pures.
 
-  wp_loadField. wp_loadField.
-  wp_apply (wp_MapGet with "HlastSeqMap").
-  iIntros (v ok) "[%HseqGet HlastSeqMap]".
   wp_pures.
-
   wp_loadField.
+  wp_apply (wp_shardOf).
   wp_pures.
+  wp_loadField.
 
-  wp_apply (wp_and_pure ok (int.Z args.(GR_Seq) ≤ int.Z v)%Z).
-  { wp_pures. by destruct ok. }
-  { iIntros "_". wp_pures. done. }
+  iDestruct (is_slice_small_acc with "HshardMap_sl") as "[HshardMap_sl HshardMap_sl_close]".
+  set (sid:=shardOfC args.(GR_Key)) in *.
+
+  assert (∃ b, shardMapping !! int.nat sid = Some b) as [? ?].
+  {
+    eapply list_lookup_lt.
+    move: HshardMapLength. rewrite /sid /shardOfC /uNSHARD.
+    word.
+  }
+  wp_apply (typed_slice.wp_SliceGet with "[$HshardMap_sl]").
+  {
+    iPureIntro. done.
+  }
+  iIntros "HshardMap_sl".
+  wp_pures.
 
   wp_if_destruct.
-  { (* reply table *)
+  { (* have the shard *)
     wp_loadField.
     wp_loadField.
-    wp_apply (map.wp_MapGet with "HlastReplyMap").
-    iIntros (reply replyOk) "[%HlookupReply HlastReplyMap]".
-    wp_pures.
-(*
-    iAssert (reply_ptr ↦[struct.t GetReply] (#_, (slice_val val_sl, #())) )%I with "[HValue HErr]" as "Hrep".
+    iDestruct (is_slice_split with "Hkvss_sl") as "[Hkvss_sl Hkvss_sl_close]".
+    iDestruct (big_sepS_elem_of_acc _ _ sid with "HownShards") as "[HownShard HownShards]".
+    { set_solver. }
+    iDestruct "HownShard" as "[%Hbad|HownShard]".
+    { exfalso. done. }
+    iDestruct "HownShard" as (kvs_ptr m mv) "(HshardGhost & %Hkvs_lookup & %Hkvs_dom & HkvsMap & HvalSlices)".
+    wp_apply (slice.wp_SliceGet _ _ _ _ _ _ _ (#kvs_ptr) with "[Hkvss_sl]").
     {
-      iApply struct_fields_split.
-      iFrame.
+      iFrame "Hkvss_sl".
+      iPureIntro.
+      rewrite list_lookup_fmap.
+      rewrite Hkvs_lookup.
       done.
     }
-*)
-    destruct ok; last first.
-    { exfalso. naive_solver. }
-    apply map_get_true in HseqGet.
-    destruct Heqb as [_ HseqLe].
+    iIntros "[Hkvss_sl %Hkvs_ty]".
 
-    (* get a copy of the is_slice for the slice we're giving in reply *)
-    assert (is_Some (lastReplyMV !! args.(GR_CID))) as [? HlastReplyMVlookup].
-    {
-      assert (args.(GR_CID) ∈ dom (gset u64) lastSeqM).
-      { by eapply elem_of_dom_2. }
-      assert (args.(GR_CID) ∈ dom (gset u64) lastReplyMV).
-      { rewrite -HlastReplyMVdom in H1. done. }
-      apply elem_of_dom.
-      done.
-    }
-
-    iDestruct (big_sepM2_lookup_iff with "HlastReply_structs") as %Hdom.
-    assert (is_Some (lastReplyM !! args.(GR_CID))) as [? HlastReplyMlookup].
-    { apply Hdom. naive_solver. }
-
-    iDestruct (big_sepM2_lookup_acc _ _ _ args.(GR_CID) with "HlastReply_structs") as "[HlastReply_struct HlastReply_structs]".
-    {
-      done.
-    }
-    {
-      done.
-    }
-
-    iDestruct "HlastReply_struct" as (srv_val_sl ?) "[%Hx Hsrv_val_sl]".
-    assert (x = reply) as ->.
-    {
-      unfold map.map_get in HlookupReply.
-      rewrite HlastReplyMVlookup in HlookupReply.
-      naive_solver.
-    }
-
-    rewrite Hx.
-    iDestruct "Hsrv_val_sl" as "[Hsrv_val_sl Hrep_val_sl]".
-    iSpecialize ("HlastReply_structs" with "[Hsrv_val_sl]").
-    {
-      iExists _, _.
-      iFrame.
-      done.
-    }
-    (* Now we have a fraction of the slice we were looking for *)
-    wp_storeField.
+    wp_apply (map.wp_MapGet with "[$HkvsMap]").
+    iIntros (value okValue) "[%HlookupVal HkvsMap]".
     wp_pures.
-    wp_storeField.
-    wp_pures.
-
-    (* now split into stale/nonstale cases. FIXME: there is still a bunch of duplication here, use lemma for if-with-merging-control-flow? *)
-    destruct (Z.lt_ge_cases (int.Z args.(GR_Seq)) (int.Z v)) as [Hcase|Hcase].
-    { (* Stale *)
-      iMod (smaller_seqno_stale_fact _ {| Req_CID:=_; Req_Seq:=_ |} v with "His_srv Hrpc") as "HH".
-      { done. }
-      { done. }
-      { done. }
-      iDestruct "HH" as "[Hrpc #Hstale]".
-      wp_loadField.
-      iApply wp_ncfupd.
-      wp_apply (release_spec with "[-HΦ HCID HSeq HKey HValue_sl HValue HErr Hrep_val_sl]").
-      {
-        iFrame "#∗".
-        iNext.
-        iExists _,_,_, _, _, _, _, _.
-        iExists _, _, _, _.
-        iFrame.
-        done.
-      }
-      wp_pures. iApply "HΦ".
-
-      iSplitL "HErr HValue Hrep_val_sl".
-      {
-        instantiate (1:={| GR_Err := _ |}).
-        iExists _; iFrame.
-        (* FIXME: we are readonly_alloc'ing several times here; we should probably push
-           this up to wherever the is_slice_small is coming from. *)
-        iMod (readonly_alloc with "[Hrep_val_sl]") as "$"; by iFrame.
-      }
-      iLeft.
-      by iFrame "#".
-    }
-    { (* Not stale *)
-      assert (v = args.(GR_Seq)) by word.
-      rewrite H1 in HseqGet.
-      iMod (server_replies_to_request _ {| Req_CID:=_; Req_Seq:=_ |} with "His_srv Hrpc") as "HH".
-      { done. }
-      { done. }
-      { eexists (mkShardReplyC 0 [] false). naive_solver. }
-
-      iDestruct "HH" as "[#Hreceipt Hrpc]".
-
-      (* prove that args.(GR_CID) is in lastReplyMV (probably just add [∗ map] _ ↦ _;_ ∈ lastReplyMV ; lastSeq, True) *)
-      wp_loadField.
-      iApply wp_ncfupd.
-      wp_apply (release_spec with "[-HΦ HCID HSeq HKey HValue_sl HValue HErr Hrep_val_sl]").
-      {
-        iFrame "#∗".
-        iNext.
-        iExists _,_,_, _, _, _, _, _.
-        iExists _, _, _, _.
-        iFrame.
-        done.
-      }
-      wp_pures. iApply "HΦ".
-      iSplitL "HErr HValue Hrep_val_sl".
-      {
-        instantiate (1:={| GR_Err := _ |}).
-        iExists _; iFrame.
-        iMod (readonly_alloc with "[Hrep_val_sl]") as "$"; by iFrame.
-      }
-      iRight.
-      rewrite HlastReplyMlookup.
-      simpl.
-      destruct x0.
-      iExists _.
-      by iFrame "#".
-    }
-  }
-  {
-    wp_loadField.
-    wp_loadField.
-    wp_loadField.
-    wp_apply (wp_MapInsert with "HlastSeqMap").
-    { done. }
-    iIntros "HlastSeqMap".
-
-    wp_pures.
-    wp_loadField.
-    wp_apply (wp_shardOf).
-    wp_pures.
-    wp_loadField.
-
-    iDestruct (is_slice_small_acc with "HshardMap_sl") as "[HshardMap_sl HshardMap_sl_close]".
-    set (sid:=shardOfC args.(GR_Key)) in *.
-
-    assert (∃ b, shardMapping !! int.nat sid = Some b) as [? ?].
-    {
-      eapply list_lookup_lt.
-      move: HshardMapLength. rewrite /sid /shardOfC /uNSHARD.
-      word.
-    }
-    wp_apply (typed_slice.wp_SliceGet with "[$HshardMap_sl]").
-    {
-      iPureIntro. done.
-    }
-    iIntros "HshardMap_sl".
-    wp_pures.
-
-    (* get resources out of escrow before splitting into cases *)
-    iMod (server_takes_request with "HreqInv Hrpc") as "HH".
-    { done. }
-    {
-      rewrite HseqGet.
-      simpl.
-      destruct ok.
-      {
-        apply map_get_true in HseqGet.
-        edestruct (Z.le_gt_cases (int.Z args.(GR_Seq)) (int.Z v)) as [Hineq|Hineq].
-        { exfalso. naive_solver. }
-        { done. }
-      }
-      {
-        apply map_get_false in HseqGet as [_ HseqGet].
-        rewrite HseqGet.
-        simpl.
-        word.
-      }
-    }
-    iDestruct "HH" as "(Hγpre & Hpre & Hproc)".
-
-    assert (int.Z v < int.Z args.(GR_Seq))%Z as HseqFresh.
-    {
-      simpl.
-      destruct ok.
-      {
-        intuition.
-        destruct (Z.le_gt_cases (int.Z args.(GR_Seq)) (int.Z v)) as [Hineq|Hineq].
-        { naive_solver. }
-        { naive_solver. }
-      }
-      {
-        apply map_get_false in HseqGet as [_ ->].
-        simpl.
-        word.
-      }
-    }
-
-    wp_if_destruct.
-    { (* have the shard *)
-      wp_loadField.
-      wp_loadField.
-      iDestruct (is_slice_split with "Hkvss_sl") as "[Hkvss_sl Hkvss_sl_close]".
-      iDestruct (big_sepS_elem_of_acc _ _ sid with "HownShards") as "[HownShard HownShards]".
-      { set_solver. }
-      iDestruct "HownShard" as "[%Hbad|HownShard]".
-      { exfalso. done. }
-      iDestruct "HownShard" as (kvs_ptr m mv) "(HshardGhost & %Hkvs_lookup & %Hkvs_dom & HkvsMap & HvalSlices)".
-      wp_apply (slice.wp_SliceGet _ _ _ _ _ _ _ (#kvs_ptr) with "[Hkvss_sl]").
-      {
-        iFrame "Hkvss_sl".
-        iPureIntro.
-        rewrite list_lookup_fmap.
-        rewrite Hkvs_lookup.
-        done.
-      }
-      iIntros "[Hkvss_sl %Hkvs_ty]".
-
-      wp_apply (map.wp_MapGet with "[$HkvsMap]").
-      iIntros (value okValue) "[%HlookupVal HkvsMap]".
-      wp_pures.
-      assert (value = default (slice_val Slice.nil) (mv !! args.(GR_Key))) as Hvalue.
-      { naive_solver. }
-      rewrite Hvalue.
-      (*
+    assert (value = default (slice_val Slice.nil) (mv !! args.(GR_Key))) as Hvalue.
+    { naive_solver. }
+    rewrite Hvalue.
+    (*
       wp_apply (typed_slice.wp_NewSlice (V:=u8)).
       iIntros (val_sl') "Hval_sl".
       rewrite Hvalue.
-       *)
+     *)
 
-      iDestruct (big_sepS_elem_of_acc _ _ args.(GR_Key) with "HvalSlices") as "[Hsrv_val_sl HvalSlices]".
-      { set_solver. }
-      iDestruct "Hsrv_val_sl" as "[%Hbad|Hsrv_val_sl]".
-      { exfalso. naive_solver. }
+    iDestruct (big_sepS_elem_of_acc _ _ args.(GR_Key) with "HvalSlices") as "[Hsrv_val_sl HvalSlices]".
+    { set_solver. }
+    iDestruct "Hsrv_val_sl" as "[%Hbad|Hsrv_val_sl]".
+    { exfalso. naive_solver. }
 
-      iDestruct "Hsrv_val_sl" as (q ?) "[%HvalSliceRe Hsrv_val_sl]".
-      rewrite HvalSliceRe.
-      (*
+    iDestruct "Hsrv_val_sl" as (q ?) "[%HvalSliceRe Hsrv_val_sl]".
+    rewrite HvalSliceRe.
+    (*
       iDestruct (typed_slice.is_slice_small_acc with "Hsrv_val_sl") as "[Hsrv_val_sl_small Hsrv_val_sl]".
-       *)
+     *)
 
-      (*
+    (*
       wp_apply (typed_slice.wp_SliceAppendSlice (V:=u8) with "[$Hval_sl $Hsrv_val_sl_small]").
 
       rewrite app_nil_l.
       iIntros (val_sl'') "[Hval_sl Hsrv_val_sl_small]".
 
       iSpecialize ("Hsrv_val_sl" with "Hsrv_val_sl_small").
-       *)
+     *)
 
-      (* fill in reply struct *)
-      wp_storeField.
-      wp_pures.
-      wp_storeField.
+    (* fill in reply struct *)
+    wp_storeField.
+    wp_pures.
+    wp_storeField.
 
-      (* save reply in reply table *)
-      wp_loadField.
-      wp_loadField.
-      wp_loadField.
-      wp_loadField.
+    wp_pures.
+    (* commit *)
+    unfold PreShardGet.
+    iApply ncfupd_wp.
+    iMod (ncfupd_mask_subseteq _) as "Hclose"; last iMod "Hpre".
+    { done. }
+    iDestruct "Hpre" as (v0) "(Hkvptsto & HfupdQ)".
+    iDestruct (own_shard_agree with "HshardGhost Hkvptsto") as %Hmatch.
+    { done. }
+    (* match up with HshardGhost *)
+    rewrite -Hmatch.
+    iMod ("HfupdQ" with "Hkvptsto") as "Q".
+    iMod "Hclose" as "_".
 
-      wp_apply (map.wp_MapInsert with "HlastReplyMap").
-      iIntros "HlastReplyMap".
+    iDestruct "Hsrv_val_sl" as "[Hsrv_val_sl Hval_sl]".
 
-      wp_pures.
-      (* commit *)
-      unfold PreShardGet.
-      iApply ncfupd_wp.
-      iMod (ncfupd_mask_subseteq _) as "Hclose"; last iMod "Hpre".
-      { done. }
-      iDestruct "Hpre" as (v0) "(Hkvptsto & HfupdQ)".
-      iDestruct (own_shard_agree with "HshardGhost Hkvptsto") as %Hmatch.
-      { done. }
-      (* match up with HshardGhost *)
-      rewrite -Hmatch.
-      iMod ("HfupdQ" with "Hkvptsto") as "Q".
-      iMod "Hclose" as "_".
-
-
-      iMod (server_completes_request with "His_srv HreqInv Hγpre [Q] Hproc") as "HH".
-      { done. }
-      { done. }
-      { rewrite HseqGet. simpl. done. }
+    iDestruct ("HshardMap_sl_close" with "HshardMap_sl") as "HshardMap_sl".
+    iModIntro.
+    wp_loadField.
+    iDestruct "Hval_sl" as "[Hrep_val_sl Hsrv_rep_val_sl]".
+    iApply wp_ncfupd.
+    wp_apply (release_spec with "[-HΦ Q Hrep_val_sl HErr HValue]").
+    {
+      iFrame "HmuInv Hlocked".
+      iNext.
+      iExists _,_,_, _, _, _.
+      iFrame.
+      iSplitL ""; first done.
+      iSplitL ""; first done.
+      iApply "HownShards".
+      iRight.
+      iExists _, _, _.
+      iFrame.
+      iSpecialize ("HvalSlices" with "[Hsrv_val_sl]").
       {
-        iNext.
-        iRight.
-        instantiate (1:=mkShardReplyC _ _ _).
-        iFrame "Q".
-        simpl.
-        done.
+        iRight. iExists _, _; iFrame. done.
       }
-      iDestruct "HH" as "(#Hreceipt & Hrpc)".
-      iModIntro.
-
-      iDestruct "Hsrv_val_sl" as "[Hsrv_val_sl Hval_sl]".
-
-      iDestruct ("HshardMap_sl_close" with "HshardMap_sl") as "HshardMap_sl".
-      wp_loadField.
-      iDestruct "Hval_sl" as "[Hrep_val_sl Hsrv_rep_val_sl]".
-      iApply wp_ncfupd.
-      wp_apply (release_spec with "[-HΦ HCID HSeq HKey Hrep_val_sl HErr HValue]").
-      {
-        iFrame "HmuInv Hlocked".
-        iNext.
-        iExists _,_,_, _, _, _, _, _.
-        iExists _, _, _, _.
-        iFrame.
-        iSplitL "".
-        {
-          iPureIntro.
-          simpl.
-          rewrite !dom_insert_L.
-          congruence.
-        }
-        iSplitL "HlastReply_structs Hsrv_rep_val_sl".
-        {
-          iApply (big_sepM2_insert_2 with "[Hsrv_rep_val_sl] HlastReply_structs").
-          { simpl.
-            iExists _, _.
-            iFrame.
-            done.
-          }
-        }
-        iSplitL ""; first done.
-        iSplitL ""; first done.
-        iApply "HownShards".
-        iRight.
-        iExists _, _, _.
-        iFrame.
-        iSpecialize ("HvalSlices" with "[Hsrv_val_sl]").
-        {
-          iRight. iExists _, _; iFrame. done.
-        }
-        iFrame "HvalSlices".
-        done.
-      }
-      wp_pures. iApply "HΦ".
-      instantiate (1:= mkGetReplyC _ _).
-      iSplitL "HErr HValue Hrep_val_sl".
-      {
-        iExists _; iFrame.
-        iMod (readonly_alloc with "[Hrep_val_sl]") as "$"; by iFrame.
-      }
-      iSimpl.
-      iRight. iExists _.
-      by iFrame "#".
+      iFrame "HvalSlices".
+      done.
     }
-    { (* don't have shard *)
-      wp_storeField.
-
-      iMod (server_completes_request with "His_srv HreqInv Hγpre [Hpre] Hproc") as "HH".
-      { done. }
-      { done. }
-      { rewrite HseqGet. simpl. done. }
-      {
-        iNext.
-        iLeft.
-        instantiate (1:=mkShardReplyC 1 dummy_rep.(GR_Value) false).
-        iFrame "Hpre".
-        simpl.
-        done.
-      }
-      iDestruct "HH" as "(#Hreceipt & Hrpc)".
-
-      wp_loadField.
-      wp_loadField.
-      wp_loadField.
-      wp_loadField.
-
-      wp_apply (map.wp_MapInsert with "HlastReplyMap").
-      iIntros "HlastReplyMap".
-      wp_pures.
-
-      wp_loadField.
-      iDestruct ("HshardMap_sl_close" with "HshardMap_sl") as "HshardMap_sl".
-      iApply wp_ncfupd.
-      wp_apply (release_spec with "[> -HΦ HCID HSeq HKey HValue HErr]").
-      {
-        iFrame "HmuInv Hlocked".
-        iMod (readonly_load with "HValue_sl") as (?) "HValue_sl'".
-        iModIntro. iNext.
-        iExists _,_,_, _, _, _, _, _.
-        iExists _, _, _, _.
-        iFrame.
-        iSplitL "".
-        { iPureIntro.
-          rewrite !dom_insert_L /=.
-          congruence. }
-        iSplitL "HlastReply_structs HValue_sl'".
-        {
-          iApply (big_sepM2_insert_2 with "[HValue_sl'] HlastReply_structs").
-          simpl.
-          iExists _, _; iFrame.
-          done.
-        }
-        done.
-      }
-      wp_pures. iModIntro. iApply "HΦ".
-      iSplitL "HErr HValue".
-      {
-        iExists _.
-        instantiate (1:=mkGetReplyC _ _).
-        by iFrame.
-      }
-      iSimpl.
-      iRight. iExists _.
-      by iFrame "#".
+    wp_pures. iApply "HΦ".
+    instantiate (1:= mkGetReplyC _ _).
+    iSplitL "HErr HValue Hrep_val_sl".
+    {
+      iExists _; iFrame.
+      iMod (readonly_alloc with "[Hrep_val_sl]") as "$"; by iFrame.
     }
+    iRight.
+    iSimpl.
+    by iFrame.
+  }
+  { (* don't have shard *)
+    wp_storeField.
+
+    wp_loadField.
+    iDestruct ("HshardMap_sl_close" with "HshardMap_sl") as "HshardMap_sl".
+    iApply wp_ncfupd.
+    wp_apply (release_spec with "[> -HΦ Hpre HValue HErr]").
+    {
+      iFrame "HmuInv Hlocked".
+      iMod (readonly_load with "HValue_sl") as (?) "HValue_sl'".
+      iModIntro. iNext.
+      iExists _,_,_, _, _, _.
+      iFrame.
+      done.
+    }
+    wp_pures. iModIntro. iApply "HΦ".
+    iSplitL "HErr HValue".
+    {
+      iExists _.
+      instantiate (1:=mkGetReplyC _ _).
+      by iFrame.
+    }
+    iLeft.
+    iSimpl.
+    by iFrame.
   }
 Qed. (* FIXME Qed takes forever, why that? *)
 
