src/program_proof/memkv/memkv_shard_start_proof.v
@@ -5,7 +5,7 @@ From Perennial.program_proof.memkv Require Export memkv_shard_definitions memkv_
 
 Section memkv_shard_start_proof.
 
-Context `{!heapGS Σ, erpcG Σ ShardReplyC, urpcregG Σ, kvMapG Σ}.
+Context `{!heapGS Σ, erpcG Σ, urpcregG Σ, kvMapG Σ}.
 
 Lemma wp_KVShardServer__Start (s:loc) (host : u64) γ :
 handlers_dom γ.(urpc_gn) {[ U64 0; U64 1; U64 2; U64 3; U64 4; U64 5 ]} -∗
@@ -24,24 +24,159 @@ Proof.
   wp_pures.
   wp_apply map.wp_NewMap.
   iIntros (handlers_ptr) "Hmap".
+  iAssert (∃ erpc, is_erpc_server γ.(erpc_gn) erpc ∗ readonly (s ↦[KVShardServer :: "erpc"] #erpc))%I as (erpc) "[#Herpc ?]".
+  { iNamed "His_memkv". eauto. }
+  wp_loadField.
   wp_pures.
+  rewrite is_shard_server_unfold.
+  iNamed "His_shard".
 
   wp_apply (map.wp_MapInsert with "Hmap").
   iIntros "Hmap".
   wp_pures.
 
+  wp_apply (wp_erpc_Server_HandleRequest (is_shard_server_putSpec γ.(kv_gn)) with "[] Herpc").
+  {
+    clear Φ.
+    iIntros ([Q req1] ?????) "!#".
+    iIntros (Φ) "Hpre HΦ".
+    wp_pures.
+    wp_apply (wp_allocStruct).
+    {
+      naive_solver.
+    }
+    iIntros (rep_ptr) "Hrep".
+    wp_pures.
+    iDestruct "Hpre" as "(Hreq_sl & Hrep_ptr & _ & [%Henc Hpre])".
+    wp_apply (wp_DecodePutRequest with "[$Hreq_sl]").
+    { done. }
+    iIntros (args_ptr val_sl) "Hargs".
+    wp_apply (wp_PutRPC with "His_memkv [$Hargs Hrep $Hpre]").
+    {
+      iDestruct (struct_fields_split with "Hrep") as "HH".
+      iNamed "HH".
+      iExists (mkPutReplyC _).
+      iFrame.
+    }
+    iIntros (rep') "[Hrep Hpost']".
+    wp_pures.
+    wp_apply (wp_EncodePutReply with "Hrep").
+    iIntros (repData rep_sl) "[Hrep_sl %HrepEnc]".
+    iDestruct (is_slice_to_small with "Hrep_sl") as "Hrep_sl".
+    wp_store.
+    iApply "HΦ". iFrame.
+    iExists _; by iFrame. 
+  }
+  iIntros (put_handler) "#Hput_handler".
   wp_apply (map.wp_MapInsert with "Hmap").
   iIntros "Hmap".
   wp_pures.
 
+  wp_apply (wp_erpc_Server_HandleRequest (is_shard_server_getSpec γ.(kv_gn)) with "[] Herpc").
+  {
+    clear Φ.
+    iIntros ([Q req1] ?????) "!#".
+    iIntros (Φ) "Hpre HΦ".
+    wp_pures.
+    wp_apply (wp_allocStruct).
+    { val_ty. }
+    iIntros (rep_ptr) "Hrep".
+    wp_pures.
+    iDestruct "Hpre" as "(Hreq_sl & Hrep_ptr & _ & [%Henc Hpre])".
+    wp_apply (wp_DecodeGetRequest with "[$Hreq_sl]").
+    { done. }
+    iIntros (args_ptr) "Hargs".
+    iDestruct (typed_slice.is_slice_zero byteT 1%Qp) as "Hzero_sl".
+    iDestruct (typed_slice.is_slice_small_acc with "Hzero_sl") as "{Hzero_sl} [Hzero_sl _]".
+    iMod (readonly_alloc_1 with "Hzero_sl") as "{Hzero_sl} Hzero_sl".
+    wp_apply (wp_GetRPC with "His_memkv [$Hargs Hrep $Hpre Hzero_sl]").
+    {
+      rewrite 2!zero_prod_val zero_slice_val.
+
+      iDestruct (struct_fields_split with "Hrep") as "HH".
+      iNamed "HH".
+      iExists (mkGetReplyC _ []).
+      iFrame.
+      iExists (Slice.nil).
+      iFrame.
+    }
+    iIntros (rep') "[Hrep Hpost']".
+    wp_pures.
+    wp_apply (wp_EncodeGetReply with "Hrep").
+    iIntros (repData rep_sl) "[Hrep_sl %HrepEnc]".
+    iDestruct (is_slice_to_small with "Hrep_sl") as "Hrep_sl".
+    wp_store.
+    iApply "HΦ". iFrame.
+    iExists _; by iFrame. 
+  }
+  iIntros (get_handler) "#Hget_handler".
   wp_apply (map.wp_MapInsert with "Hmap").
   iIntros "Hmap".
   wp_pures.
 
+  wp_apply (wp_erpc_Server_HandleRequest (is_shard_server_conditionalPutSpec γ.(kv_gn)) with "[] Herpc").
+  {
+      clear Φ.
+      iIntros ([Q req1] ?????) "!#".
+      iIntros (Φ) "Hpre HΦ".
+      wp_pures.
+      wp_apply (wp_allocStruct).
+      {
+        naive_solver.
+      }
+      iIntros (rep_ptr) "Hrep".
+      wp_pures.
+      iDestruct "Hpre" as "(Hreq_sl & Hrep_ptr & _ & [%Henc Hpre])".
+      wp_apply (wp_DecodeConditionalPutRequest with "[$Hreq_sl]").
+      { done. }
+      iIntros (args_ptr expv_sl newv) "Hargs".
+      wp_apply (wp_ConditionalPutRPC with "His_memkv [$Hargs $Hpre Hrep]").
+      {
+        iDestruct (struct_fields_split with "Hrep") as "HH".
+        iNamed "HH".
+        iExists (mkConditionalPutReplyC _ _).
+        iFrame.
+      }
+      iIntros (rep') "[Hrep Hpost']".
+      wp_pures.
+      wp_apply (wp_EncodeConditionalPutReply with "Hrep").
+      iIntros (repData rep_sl) "[Hrep_sl %HrepEnc]".
+      iDestruct (is_slice_to_small with "Hrep_sl") as "Hrep_sl".
+      wp_store.
+      iApply "HΦ". iFrame. iSimpl.
+      iExists _; by iFrame.
+  }
+  iIntros (cput_handler) "#Hcput_handler".
   wp_apply (map.wp_MapInsert with "Hmap").
   iIntros "Hmap".
   wp_pures.
 
+  wp_apply (wp_erpc_Server_HandleRequest (is_shard_server_installSpec γ.(kv_gn)) with "[] Herpc").
+  {
+    clear Φ.
+    iIntros ([] ?????) "!#".
+    iIntros (Φ) "Hpre HΦ".
+    wp_pures.
+
+    iDestruct "Hpre" as "(Hpre_sl & Hrep & _ & Hpre)".
+    iDestruct "Hpre" as (?) "(%Hargs_enc & %HsidLe & Hshard)".
+    wp_apply (wp_decodeInstallShardRequest with "[$Hpre_sl]").
+    { done. }
+    iIntros (args_ptr) "Hargs".
+    wp_apply (wp_InstallShardRPC with "His_memkv [$Hargs $Hshard]").
+    {
+      iPureIntro.
+      word.
+    }
+    wp_pures.
+    wp_apply (typed_slice.wp_NewSlice (V:=u8)).
+    iIntros (reply_sl) "Hrep_sl".
+    iDestruct (is_slice_to_small with "Hrep_sl") as "Hrep_sl".
+    wp_store.
+    iApply "HΦ".
+    iFrame. done.
+  }
+  iIntros (install_handler) "#Hinstall_handler".
   wp_apply (map.wp_MapInsert with "Hmap").
   iIntros "Hmap".
   wp_pures.
@@ -54,8 +189,6 @@ Proof.
   iIntros (rs) "Hsown".
   wp_pures.
 
-  rewrite is_shard_server_unfold.
-  iNamed "His_shard".
   wp_apply (wp_StartServer with "[$Hsown]").
   { rewrite ?dom_insert_L; set_solver. }
   {
@@ -89,159 +222,22 @@ Proof.
     }
 
     iApply (big_sepM_insert_2 with "").
-    { (* InstallShard() handler_is *)
-      iExists _.
-      iFrame "#HinstallSpec".
-
-      clear Φ.
-      iIntros (??????) "!#".
-      iIntros (Φ) "Hpre HΦ".
-      wp_pures.
-
-      iDestruct "Hpre" as "(Hpre_sl & Hrep & _ & Hpre)".
-      iDestruct "Hpre" as (x) "[Hpre Hpost]".
-      iDestruct "Hpre" as (?) "(%Hargs_enc & %HsidLe & HreqInv)".
-      wp_apply (wp_decodeInstallShardRequest with "[$Hpre_sl]").
-      { done. }
-      iIntros (args_ptr) "Hargs".
-      wp_apply (wp_InstallShardRPC with "His_memkv [$Hargs $HreqInv]").
-      {
-        iPureIntro.
-        word.
-      }
-      wp_pures.
-      wp_apply (typed_slice.wp_NewSlice (V:=u8)).
-      iIntros (reply_sl) "Hrep_sl".
-      iDestruct (is_slice_to_small with "Hrep_sl") as "Hrep_sl".
-      wp_store.
-      iApply "HΦ".
-      iFrame.
-      iApply "Hpost". by iFrame.
+    { iExists _. iFrame "HinstallSpec Hinstall_handler".
     }
 
     iApply (big_sepM_insert_2 with "").
     { (* ConditionalPutRPC handler_is *)
-      simpl.
-      iExists _. iFrame "HconditionalPutSpec".
-
-      clear Φ.
-      iIntros (??????) "!#".
-      iIntros (Φ) "Hpre HΦ".
-      wp_pures.
-      wp_apply (wp_allocStruct).
-      {
-        naive_solver.
-      }
-      iIntros (rep_ptr) "Hrep".
-      wp_pures.
-      iDestruct "Hpre" as "(Hreq_sl & Hrep_ptr & _ & Hpre)".
-      iSimpl in "Hpre". iDestruct "Hpre" as ([[Q γreq] req1]) "[Hpre Hpost]".
-      iDestruct "Hpre" as "(%Henc & #HreqInv)".
-      wp_apply (wp_DecodeConditionalPutRequest with "[$Hreq_sl]").
-      { done. }
-      iIntros (args_ptr expv_sl newv) "Hargs".
-      wp_apply (wp_ConditionalPutRPC with "His_memkv [$Hargs Hrep HreqInv]").
-      {
-        iFrame "HreqInv".
-        iDestruct (struct_fields_split with "Hrep") as "HH".
-        iNamed "HH".
-        iExists (mkConditionalPutReplyC _ _).
-        iFrame.
-      }
-      iIntros (rep') "[Hrep Hpost']".
-      wp_pures.
-      wp_apply (wp_EncodeConditionalPutReply with "Hrep").
-      iIntros (repData rep_sl) "[Hrep_sl %HrepEnc]".
-      iDestruct (is_slice_to_small with "Hrep_sl") as "Hrep_sl".
-      wp_store.
-      iApply "HΦ". iFrame. iApply "Hpost".
-      iModIntro.
-      iExists _; by iFrame.
+      iExists _. iFrame "HconditionalPutSpec Hcput_handler".
     }
 
     iApply (big_sepM_insert_2 with "").
     { (* Get() handler_is *)
-      simpl.
-      iExists _; iFrame "HgetSpec".
-
-      clear Φ.
-      iIntros (??????) "!#".
-      iIntros (Φ) "Hpre HΦ".
-      wp_pures.
-      wp_apply (wp_allocStruct).
-      { val_ty. }
-      iIntros (rep_ptr) "Hrep".
-      wp_pures.
-      iDestruct "Hpre" as "(Hreq_sl & Hrep_ptr & _ & Hpre)".
-      iSimpl in "Hpre". iDestruct "Hpre" as ([[Q γreq] req1]) "[Hpre Hpost]".
-      iDestruct "Hpre" as "(%Henc & #HreqInv)".
-      wp_apply (wp_DecodeGetRequest with "[$Hreq_sl]").
-      { done. }
-      iIntros (args_ptr) "Hargs".
-      iDestruct (typed_slice.is_slice_zero byteT 1%Qp) as "Hzero_sl".
-      iDestruct (typed_slice.is_slice_small_acc with "Hzero_sl") as "{Hzero_sl} [Hzero_sl _]".
-      iMod (readonly_alloc_1 with "Hzero_sl") as "{Hzero_sl} Hzero_sl".
-      wp_apply (wp_GetRPC with "His_memkv [$Hargs Hrep HreqInv Hzero_sl]").
-      {
-        iFrame "HreqInv".
-        rewrite 2!zero_prod_val zero_slice_val.
-
-        iDestruct (struct_fields_split with "Hrep") as "HH".
-        iNamed "HH".
-        iExists (mkGetReplyC _ []).
-        iFrame.
-        iExists (Slice.nil).
-        iFrame.
-      }
-      iIntros (rep') "[Hrep Hpost']".
-      wp_pures.
-      wp_apply (wp_EncodeGetReply with "Hrep").
-      iIntros (repData rep_sl) "[Hrep_sl %HrepEnc]".
-      iDestruct (is_slice_to_small with "Hrep_sl") as "Hrep_sl".
-      wp_store.
-      iApply "HΦ". iFrame. iApply "Hpost".
-      iModIntro.
-      iExists _; by iFrame.
+      iExists _; iFrame "HgetSpec Hget_handler".
     }
 
     iApply (big_sepM_insert_2 with "").
     { (* PutRPC handler_is *)
-      simpl.
-      iExists _. iFrame "HputSpec".
-
-      clear Φ.
-      iIntros (??????) "!#".
-      iIntros (Φ) "Hpre HΦ".
-      wp_pures.
-      wp_apply (wp_allocStruct).
-      {
-        naive_solver.
-      }
-      iIntros (rep_ptr) "Hrep".
-      wp_pures.
-      iDestruct "Hpre" as "(Hreq_sl & Hrep_ptr & _ & Hpre)".
-      iSimpl in "Hpre". iDestruct "Hpre" as ([[Q γreq] req1]) "[Hpre Hpost]".
-      iDestruct "Hpre" as "(%Henc & #HreqInv)".
-      wp_apply (wp_DecodePutRequest with "[$Hreq_sl]").
-      { done. }
-      iIntros (args_ptr val_sl) "Hargs".
-      wp_apply (wp_PutRPC with "His_memkv [$Hargs Hrep HreqInv]").
-      {
-        iFrame "HreqInv".
-        iDestruct (struct_fields_split with "Hrep") as "HH".
-        iNamed "HH".
-        iExists (mkPutReplyC _).
-        iFrame.
-      }
-      iIntros (rep') "[Hrep Hpost']".
-      wp_pures.
-      wp_apply (wp_EncodePutReply with "Hrep").
-      iIntros (repData rep_sl) "[Hrep_sl %HrepEnc]".
-      iDestruct (is_slice_to_small with "Hrep_sl") as "Hrep_sl".
-      wp_store.
-      iApply "HΦ". iFrame. iApply "Hpost".
-      iModIntro.
-      iExists _; by iFrame.
+      iExists _. iFrame "HputSpec Hput_handler".
     }
 
     iApply (big_sepM_insert_2 with "").
@@ -249,7 +245,7 @@ Proof.
       iExists _.
       iFrame "HfreshSpec".
 
-      clear Φ.
+      clear Φ. rewrite /impl_handler_spec.
       iIntros (??????) "!#".
       iIntros (Φ) "Hpre HΦ".
       wp_pures.
